feat: unique typing proved 🎉 (modulo injectivity)

Lean4Lean/Theory/Typing/Strong.lean
@@ -7,9 +7,11 @@ open VExpr
 
 section
 set_option hygiene false
+variable (env : VEnv) (uvars : Nat)
+
+section
 local notation:65 Γ " ⊢ " e " : " A:30 => IsDefEqStrong Γ e e A
 local notation:65 Γ " ⊢ " e1 " ≡ " e2 " : " A:30 => IsDefEqStrong Γ e1 e2 A
-variable (env : VEnv) (uvars : Nat)
 
 inductive IsDefEqStrong : List VExpr → VExpr → VExpr → VExpr → Prop where
   | bvar : Lookup Γ i A → u.WF uvars → Γ ⊢ A : .sort u → Γ ⊢ .bvar i : A
@@ -25,10 +27,8 @@ inductive IsDefEqStrong : List VExpr → VExpr → VExpr → VExpr → Prop wher
     ls.length = ci.uvars →
     List.Forall₂ (· ≈ ·) ls ls' →
     u.WF uvars →
-    [] ⊢ ci.type.instL ls : .sort u →
-    [] ⊢ ci.type.instL ls' : .sort u →
-    Γ ⊢ ci.type.instL ls : .sort u →
-    Γ ⊢ ci.type.instL ls' : .sort u →
+    [] ⊢ ci.type.instL ls ≡ ci.type.instL ls' : .sort u →
+    Γ ⊢ ci.type.instL ls ≡ ci.type.instL ls' : .sort u →
     Γ ⊢ .const c ls ≡ .const c ls' : ci.type.instL ls
   | appDF :
     u.WF uvars → v.WF uvars →
@@ -67,6 +67,7 @@ inductive IsDefEqStrong : List VExpr → VExpr → VExpr → VExpr → Prop wher
     A.lift::A::Γ ⊢ B.liftN 1 1 : .sort v →
     Γ ⊢ e : .forallE A B →
     A::Γ ⊢ e.lift : .forallE A.lift (B.liftN 1 1) →
+    A::Γ ⊢ A.lift : .sort u →
     Γ ⊢ .lam A (.app e.lift (.bvar 0)) ≡ e : .forallE A B
   | proofIrrel :
     Γ ⊢ p : .sort .zero → Γ ⊢ h : p → Γ ⊢ h' : p →
@@ -83,6 +84,55 @@ inductive IsDefEqStrong : List VExpr → VExpr → VExpr → VExpr → Prop wher
 
 end
 
+section
+local notation:65 Γ " ⊢ " e " : " A:30 => HasTypeStrong Γ e A true
+local notation:65 Γ " ⊢ " e " :! " A:30 => HasTypeStrong Γ e A false
+local notation:65 Γ " ⊢ " e1 " ≡ " e2 " : " A:30 => IsDefEqStrong env uvars Γ e1 e2 A
+
+/--
+This is functionally a mutual inductive type,
+but using a bool index makes it easier to do induction in lean.
+The defeq rule is separated from the structural rules for easy inversion.
+-/
+inductive HasTypeStrong : List VExpr → VExpr → VExpr → Bool → Prop where
+  | bvar : Lookup Γ i A → u.WF uvars → Γ ⊢ A : .sort u → Γ ⊢ .bvar i :! A
+  | sort' : l.WF uvars → l'.WF uvars → l ≈ l' → Γ ⊢ .sort l :! .sort (.succ l')
+  | const :
+    env.constants c = some ci →
+    (∀ l ∈ ls, l.WF uvars) →
+    ls.length = ci.uvars →
+    u.WF uvars →
+    [] ⊢ ci.type.instL ls : .sort u →
+    Γ ⊢ ci.type.instL ls : .sort u →
+    Γ ⊢ .const c ls :! ci.type.instL ls
+  | app :
+    u.WF uvars → v.WF uvars →
+    Γ ⊢ A : .sort u →
+    A::Γ ⊢ B : .sort v →
+    Γ ⊢ .forallE A B : .sort (.imax u v) →
+    Γ ⊢ f : .forallE A B →
+    Γ ⊢ a : A →
+    Γ ⊢ B.inst a : .sort v →
+    Γ ⊢ .app f a :! B.inst a
+  | lam :
+    u.WF uvars → v.WF uvars →
+    Γ ⊢ A : .sort u →
+    A::Γ ⊢ B : .sort v →
+    A::Γ ⊢ body : B →
+    Γ ⊢ .forallE A B : .sort (.imax u v) →
+    Γ ⊢ .lam A body :! .forallE A B
+  | forallE :
+    u.WF uvars → v.WF uvars →
+    Γ ⊢ A : .sort u →
+    A::Γ ⊢ body : .sort v →
+    Γ ⊢ .forallE A body :! .sort (.imax u v)
+  | base : Γ ⊢ e :! A → Γ ⊢ e : A
+  | defeq : u.WF uvars → Γ ⊢ A ≡ B : .sort u →
+    Γ ⊢ A : .sort u → Γ ⊢ B : .sort u → Γ ⊢ e : A → Γ ⊢ e : B
+end
+
+end
+
 theorem IsDefEqStrong.hasType {env : VEnv}
     (H : env.IsDefEqStrong U Γ e1 e2 A) :
     env.IsDefEqStrong U Γ e1 e1 A ∧ env.IsDefEqStrong U Γ e2 e2 A :=
@@ -96,9 +146,9 @@ theorem IsDefEqStrong.weakN (W : Ctx.LiftN n k Γ Γ') (H : env.IsDefEqStrong U 
   | symm _ ih => exact .symm (ih W)
   | trans _ _ ih1 ih2 => exact .trans (ih1 W) (ih2 W)
   | sortDF h1 h2 h3 => exact .sortDF h1 h2 h3
-  | constDF h1 h2 h3 h4 h5 h6 h7 h8 _ _ _ _ ih3 ih4 =>
-    simp [(henv.closedC h1).instL.liftN_eq (Nat.zero_le _)] at ih3 ih4 ⊢
-    exact .constDF h1 h2 h3 h4 h5 h6 h7 h8 (ih3 W) (ih4 W)
+  | constDF h1 h2 h3 h4 h5 h6 h7 _ _ ih2 =>
+    simp [(henv.closedC h1).instL.liftN_eq (Nat.zero_le _)] at ih2 ⊢
+    exact .constDF h1 h2 h3 h4 h5 h6 h7 (ih2 W)
   | appDF h1 h2 _ _ _ _ _ ih1 ih2 ih3 ih4 ih5 =>
     refine liftN_inst_hi .. ▸ .appDF h1 h2 (ih1 W) (ih2 W.succ) (ih3 W) (ih4 W) ?_
     exact liftN_inst_hi .. ▸ liftN_inst_hi .. ▸ ih5 W
@@ -111,14 +161,16 @@ theorem IsDefEqStrong.weakN (W : Ctx.LiftN n k Γ Γ') (H : env.IsDefEqStrong U 
       (ih1 W) (ih2 W.succ) (ih3 W.succ) (ih4 W)
       (liftN_instN_hi .. ▸ ih5 W :)
       (liftN_instN_hi .. ▸ liftN_instN_hi .. ▸ ih6 W :)
-  | @eta Γ a u B v e h1 h2 _ _ _ _ _ ih1 ih2 ih3 ih4 ih5 =>
-    have := IsDefEqStrong.eta h1 h2 (ih1 W) (ih2 W.succ) ?_ (ih4 W) ?_
+  | @eta Γ a u B v e h1 h2 _ _ _ _ _ _ ih1 ih2 ih3 ih4 ih5 ih6 =>
+    have := IsDefEqStrong.eta h1 h2 (ih1 W) (ih2 W.succ) ?_ (ih4 W) ?_ ?_
     · simp [liftN]; rwa [← lift_liftN']
     · specialize ih3 W.succ.succ
       have := liftN'_comm B n 1 (k+1) 1 (Nat.le_add_left ..)
       rw [Nat.add_comm 1] at this; rwa [← this, ← lift_liftN'] at ih3
     · have ih5 : IsDefEqStrong _ _ _ _ _ (liftN n (lift (forallE ..)) _) := ih5 W.succ
       rwa [← lift_liftN', ← lift_liftN'] at ih5
+    · have ih6 := ih6 W.succ
+      rwa [← lift_liftN'] at ih6
   | proofIrrel _ _ _ ih1 ih2 ih3 => exact .proofIrrel (ih1 W) (ih2 W) (ih3 W)
   | extra h1 h2 h3 h4 h5 h6 h7 _ _ _ _ _ ih4 ih5 =>
     have ⟨⟨hA1, _⟩, hA2, hA3⟩ := henv.closed.2 h1
@@ -140,7 +192,7 @@ theorem IsDefEqStrong.defeq (H : IsDefEqStrong env U Γ e1 e2 A) : env.IsDefEq U
   | forallEDF _ _ _ _ _ ih1 ih2 => exact .forallEDF ih1 ih2
   | defeqDF _ _ _ ih1 ih2 => exact .defeqDF ih1 ih2
   | beta _ _ _ _ _ _ _ _ _ _ ih1 ih2 => exact .beta ih1 ih2
-  | eta _ _ _ _ _ _ _ _ _ _ ih => exact .eta ih
+  | eta _ _ _ _ _ _ _ _ _ _ _ ih => exact .eta ih
   | proofIrrel _ _ _ ih1 ih2 ih3 => exact .proofIrrel ih1 ih2 ih3
   | extra h1 h2 h3 => exact .extra h1 h2 h3
 
@@ -152,14 +204,14 @@ theorem IsDefEqStrong.mono
   | symm _ ih => exact .symm ih
   | trans _ _ ih1 ih2 => exact .trans ih1 ih2
   | sortDF h1 h2 h3 => exact .sortDF h1 h2 h3
-  | constDF h1 h2 h3 h4 h5 h6 _ _ _ _ ih1 ih2 ih3 ih4 =>
-    exact .constDF (henv.1 h1) h2 h3 h4 h5 h6 ih1 ih2 ih3 ih4
+  | constDF h1 h2 h3 h4 h5 h6 _ _ ih1 ih2 =>
+    exact .constDF (henv.1 h1) h2 h3 h4 h5 h6 ih1 ih2
   | appDF h1 h2 _ _ _ _ _ ih1 ih2 ih3 ih4 ih5 => exact .appDF h1 h2 ih1 ih2 ih3 ih4 ih5
   | lamDF h1 h2  _ _ _ _ _ ih1 ih2 ih3 ih4 ih5 => exact .lamDF h1 h2 ih1 ih2 ih3 ih4 ih5
   | forallEDF h1 h2 _ _ _ ih1 ih2 ih3 => exact .forallEDF h1 h2 ih1 ih2 ih3
   | defeqDF h1 _ _ ih1 ih2 => exact .defeqDF h1 ih1 ih2
   | beta h1 h2 _ _ _ _ _ _ ih1 ih2 ih3 ih4 ih5 ih6 => exact .beta h1 h2 ih1 ih2 ih3 ih4 ih5 ih6
-  | eta h1 h2 _ _ _ _ _ ih1 ih2 ih3 ih4 ih5 => exact .eta h1 h2 ih1 ih2 ih3 ih4 ih5
+  | eta h1 h2 _ _ _ _ _ _ ih1 ih2 ih3 ih4 ih5 ih6 => exact .eta h1 h2 ih1 ih2 ih3 ih4 ih5 ih6
   | proofIrrel _ _ _ ih1 ih2 ih3 => exact .proofIrrel ih1 ih2 ih3
   | extra h1 h2 h3 h4 _ _ _ _ _ ih1 ih2 ih3 ih4 ih5 =>
     exact .extra (henv.2 h1) h2 h3 h4 ih1 ih2 ih3 ih4 ih5
@@ -171,17 +223,88 @@ theorem IsDefEqStrong.weak0 (H : env.IsDefEqStrong U [] e1 e2 A) :
   simpa [h1.liftN_eq (Nat.zero_le _), h2.liftN_eq (Nat.zero_le _),
     h3.liftN_eq (Nat.zero_le _)] using H.weakN henv (.zero Γ rfl)
 
+inductive EqUpToLevels (U : Nat) : VExpr → VExpr → Prop
+  | bvar : EqUpToLevels U (.bvar i) (.bvar i)
+  | const : (∀ l ∈ ls, l.WF U) → (∀ l ∈ ls', l.WF U) → List.Forall₂ (· ≈ ·) ls ls' →
+    EqUpToLevels U (.const c ls) (.const c ls')
+  | sort : l.WF U → l'.WF U → l ≈ l' → EqUpToLevels U (.sort l) (.sort l')
+  | app : EqUpToLevels U f f' → EqUpToLevels U a a' → EqUpToLevels U (.app f a) (.app f' a')
+  | lam : EqUpToLevels U A A' → EqUpToLevels U e e' → EqUpToLevels U (.lam A e) (.lam A' e')
+  | forallE : EqUpToLevels U A A' → EqUpToLevels U B B' → EqUpToLevels U (.forallE A B) (.forallE A' B')
+
+variable! {env : VEnv} {ls ls' : List VLevel}
+    (hls : ∀ l ∈ ls, l.WF U) (hls' : ∀ l ∈ ls', l.WF U) (heq : List.Forall₂ (· ≈ ·) ls ls') in
+theorem EqUpToLevels.instL (H : env.IsDefEqStrong U' Γ e1 e2 A) :
+    EqUpToLevels U (e1.instL ls) (e1.instL ls') ∧ EqUpToLevels U (e2.instL ls) (e2.instL ls') := by
+  induction H with
+  | bvar => exact ⟨.bvar, .bvar⟩
+  | symm _ ih => exact ih.symm
+  | trans _ _ ih1 ih2 | proofIrrel _ _  _ _ ih1 ih2
+  | extra _ _ _ _ _ _ _ _ _ _ ih1 ih2 => exact ⟨ih1.1, ih2.2⟩
+  | sortDF h1 h2 h3 =>
+    constructor <;> exact .sort (.inst hls) (.inst hls') (VLevel.inst_congr rfl heq)
+  | constDF h1 h2 h3 h4 h5 =>
+    constructor <;> exact .const
+      (List.forall_mem_map.2 fun _ _ => .inst hls)
+      (List.forall_mem_map.2 fun _ _ => .inst hls')
+      (List.forall₂_map_left_iff.2 <| List.forall₂_map_right_iff.2 <|
+        .rfl fun _ _ => VLevel.inst_congr rfl heq)
+  | appDF _ _ _ _ _ _ _ _ _ ih1 ih2 => exact ⟨.app ih1.1 ih2.1, .app ih1.2 ih2.2⟩
+  | lamDF _ _ _ _ _ _ _ ih1 _ _ ih2 => exact ⟨.lam ih1.1 ih2.1, .lam ih1.2 ih2.2⟩
+  | forallEDF _ _ _ _ _ ih1 ih2 => exact ⟨.forallE ih1.1 ih2.1, .forallE ih1.2 ih2.2⟩
+  | defeqDF _ _ _ _ ih => exact ih
+  | beta _ _ _ _ _ _ _ _ ih1 _ ih3 ih4 _ ih6 => exact ⟨.app (.lam ih1.1 ih3.1) ih4.1, ih6.2⟩
+  | eta _ _ _ _ _ _ _ _ ih1 _ _ ih4 ih5 => exact ⟨.lam ih1.1 (.app ih5.1 .bvar), ih4.1⟩
+
+
+variable! {env : VEnv} (W : OnCtx Γ fun _ A => A.LevelWF U) in
+theorem EqUpToLevels.refl (H : env.IsDefEqStrong U Γ e1 e2 A) :
+    EqUpToLevels U e1 e1 ∧ EqUpToLevels U e2 e2 := by
+  have := IsDefEq.levelWF H.defeq W
+  exact LevelWF.instL_id this.1 ▸ LevelWF.instL_id this.2.1 ▸
+    EqUpToLevels.instL VLevel.params_wf VLevel.params_wf (.rfl fun _ _ => rfl) H
+
+theorem EqUpToLevels.weakN (H : EqUpToLevels U e e') :
+    EqUpToLevels U (e.liftN n k) (e'.liftN n k) := by
+  induction H generalizing k with
+  | bvar => exact .bvar
+  | const h1 h2 h3 => exact .const h1 h2 h3
+  | sort h1 h2 h3 => exact .sort h1 h2 h3
+  | app _ _ ih1 ih2 => exact .app ih1 ih2
+  | lam _ _ ih1 ih2 => exact .lam ih1 ih2
+  | forallE _ _ ih1 ih2 => exact .forallE ih1 ih2
+
+variable! (h₀ : EqUpToLevels U e₀ e₀') in
+theorem EqUpToLevels.instN (H : EqUpToLevels U e e') :
+    EqUpToLevels U (e.inst e₀ k) (e'.inst e₀' k) := by
+  induction H generalizing k with
+  | bvar => simp [inst, instVar]; split <;> [exact .bvar; split] <;> [exact h₀.weakN; exact .bvar]
+  | const h1 h2 h3 => exact .const h1 h2 h3
+    | sort h1 h2 h3 => exact .sort h1 h2 h3
+  | app _ _ ih1 ih2 => exact .app ih1 ih2
+  | lam _ _ ih1 ih2 => exact .lam ih1 ih2
+  | forallE _ _ ih1 ih2 => exact .forallE ih1 ih2
+
+def EnvStrong (env : VEnv) (U : Nat) (e A : VExpr) : Prop :=
+  env.IsDefEqStrong U [] e e A ∧
+  (∃ u, env.IsDefEqStrong U [] A A (.sort u)) ∧
+  (∀ U' ls ls', (∀ l ∈ ls, l.WF U') → (∀ l ∈ ls', l.WF U') → List.Forall₂ (· ≈ ·) ls ls' →
+    env.IsDefEqStrong U' [] (e.instL ls) (e.instL ls') (A.instL ls)) ∧
+  ∀ A B, e = A.forallE B →
+    (∃ u, env.IsDefEqStrong U [] A A (.sort u)) ∧
+    (∃ u, env.IsDefEqStrong U [A] B B (.sort u))
+
 variable! {env : VEnv} {ls : List VLevel} (hls : ∀ l ∈ ls, l.WF U') in
 theorem IsDefEqStrong.instL (H : env.IsDefEqStrong U Γ e1 e2 A) :
     env.IsDefEqStrong U' (Γ.map (VExpr.instL ls)) (e1.instL ls) (e2.instL ls) (A.instL ls) := by
   induction H with
   | bvar h _ _ ih =>
     exact .bvar h.instL (.inst hls) ih
-  | constDF h1 h2 h3 h4 h5 _ _ _ _ _ ih1 ih2 ih3 ih4 =>
-    simp [VExpr.instL, VExpr.instL_instL] at ih1 ih2 ih3 ih4 ⊢
+  | constDF h1 h2 h3 h4 h5 _ _ _ ih1 ih2 =>
+    simp [VExpr.instL, VExpr.instL_instL] at ih1 ih2 ⊢
     exact .constDF h1
       (by simp [VLevel.WF.inst hls]) (by simp [VLevel.WF.inst hls]) (by simp [h4])
-      (by simpa using h5.imp fun _ _ => VLevel.inst_congr_l) (.inst hls) ih1 ih2 ih3 ih4
+      (by simpa using h5.imp fun _ _ => VLevel.inst_congr_l) (.inst hls) ih1 ih2
   | symm _ ih => exact .symm ih
   | trans _ _ ih1 ih2 => exact .trans ih1 ih2
   | sortDF _ _ h3 =>
@@ -198,9 +321,9 @@ theorem IsDefEqStrong.instL (H : env.IsDefEqStrong U Γ e1 e2 A) :
   | beta _ _ _ _ _ _ _ _ ih1 ih2 ih3 ih4 ih5 ih6 =>
     simpa using .beta (.inst hls) (.inst hls) ih1 ih2 ih3 ih4
       (by simpa using ih5) (by simpa using ih6)
-  | eta _ _ _ _ _ _ _ ih1 ih2 ih3 ih4 ih5 =>
+  | eta _ _ _ _ _ _ _ _ ih1 ih2 ih3 ih4 ih5 ih6 =>
     simpa [VExpr.instL] using .eta (.inst hls) (.inst hls) ih1 ih2
-      (by simpa using ih3) ih4 (by simpa [VExpr.instL] using ih5)
+      (by simpa using ih3) ih4 (by simpa [VExpr.instL] using ih5) (by simpa [VExpr.instL] using ih6)
   | proofIrrel _ _ _ ih1 ih2 ih3 =>
     exact .proofIrrel ih1 ih2 ih3
   | extra h1 h2 h3 _ _ _ _ _ _ ih1 ih2 ih3 ih4 ih5 =>
@@ -218,6 +341,10 @@ nonrec theorem CtxStrong.lookup {Γ} (H : CtxStrong env U Γ) (h : Lookup Γ i A
 
 theorem CtxStrong.defeq {Γ} (H : CtxStrong env U Γ) : OnCtx Γ (env.IsType U) :=
   H.mono fun ⟨_, h⟩ => ⟨_, h.defeq⟩
+
+theorem CtxStrong.levelWF : ∀ {Γ}, CtxStrong env U Γ → OnCtx Γ fun _ A => A.LevelWF U
+  | [], h => h
+  | _::_, ⟨h1, _, h2⟩ => ⟨levelWF h1, (h2.defeq.levelWF (levelWF h1)).1⟩
 
 variable! (henv : Ordered env) (h₀ : env.IsDefEqStrong U Γ₀ e₀ e₀ A₀) (hΓ₀ : CtxStrong env U Γ₀) in
 theorem IsDefEqStrong.instN (W : Ctx.InstN Γ₀ e₀ A₀ k Γ₁ Γ) (H : env.IsDefEqStrong U Γ₁ e1 e2 A)
@@ -242,9 +369,9 @@ theorem IsDefEqStrong.instN (W : Ctx.InstN Γ₀ e₀ A₀ k Γ₁ Γ) (H : env.
   | symm _ ih => exact .symm (ih W hΓ)
   | trans _ _ ih1 ih2 => exact .trans (ih1 W hΓ) (ih2 W hΓ)
   | sortDF h1 h2 h3 => exact .sortDF h1 h2 h3
-  | constDF h1 h2 h3 h4 h5 h6 h7 h8 _ _ _ _ ih3 ih4 =>
-    simp [(henv.closedC h1).instL.instN_eq (Nat.zero_le _)] at ih3 ih4 ⊢
-    exact .constDF h1 h2 h3 h4 h5 h6 h7 h8 (ih3 W hΓ) (ih4 W hΓ)
+  | constDF h1 h2 h3 h4 h5 h6 h7 _ _ ih2 =>
+    simp [(henv.closedC h1).instL.instN_eq (Nat.zero_le _)] at ih2 ⊢
+    exact .constDF h1 h2 h3 h4 h5 h6 h7 (ih2 W hΓ)
   | appDF h1 h2 _ _ _ _ _ ih1 ih2 ih3 ih4 ih5 =>
     exact inst0_inst_hi .. ▸ .appDF h1 h2
       (ih1 W hΓ) (ih2 W.succ ⟨hΓ, _, ih1 W hΓ⟩)
@@ -264,7 +391,7 @@ theorem IsDefEqStrong.instN (W : Ctx.InstN Γ₀ e₀ A₀ k Γ₁ Γ) (H : env.
       .beta h1 h2
         (ih1 W hΓ) (ih2 W.succ hΓ') (ih3 W.succ hΓ') (ih4 W hΓ)
         (inst0_inst_hi .. ▸ ih5 W hΓ) (inst0_inst_hi .. ▸ inst0_inst_hi .. ▸ ih6 W hΓ)
-  | eta h1 h2 _ _ _ _ _ ih1 ih2 ih3 ih4 ih5 =>
+  | eta h1 h2 _ _ _ _ _ _ ih1 ih2 ih3 ih4 ih5 ih6 =>
     have :=
       have hΓ' := ⟨hΓ, _, (ih1 W hΓ).hasType.1⟩
       IsDefEqStrong.eta h1 h2 (ih1 W hΓ) (ih2 W.succ hΓ')
@@ -277,6 +404,7 @@ theorem IsDefEqStrong.instN (W : Ctx.InstN Γ₀ e₀ A₀ k Γ₁ Γ) (H : env.
           have := ih5 W.succ hΓ'
           simp only [inst, ← lift_instN_lo] at this
           rwa [liftN_instN_lo (hj := Nat.le_add_left ..), Nat.add_comm 1])
+        (by simpa [inst, ← lift_instN_lo] using ih6 W.succ hΓ')
     rw [lift, liftN_instN_lo (hj := Nat.zero_le _), Nat.add_comm] at this
     simpa [inst]
   | proofIrrel _ _ _ ih1 ih2 ih3 => exact .proofIrrel (ih1 W hΓ) (ih2 W hΓ) (ih3 W hΓ)
@@ -297,13 +425,6 @@ theorem IsDefEqStrong.defeqDF_l (henv : Ordered env) (hΓ : CtxStrong env U Γ)
     h1.weakN henv (.one (A := A'))
       |>.symm.defeqDF hu (.bvar .zero hu (h1.hasType.2.weakN henv .one))
       |>.instN henv hΓ' .zero (h2.weakN henv (.succ (.one (A := A')))) hΓ'
-
-def EnvStrong (env : VEnv) (U : Nat) (e A : VExpr) : Prop :=
-  env.IsDefEqStrong U [] e e A ∧
-  (∃ u, env.IsDefEqStrong U [] A A (.sort u)) ∧
-  ∀ A B, e = A.forallE B →
-    (∃ u, env.IsDefEqStrong U [] A A (.sort u)) ∧
-    (∃ u, env.IsDefEqStrong U [A] B B (.sort u))
 
 variable! (henv : Ordered env) (envIH : env.OnTypes (EnvStrong env)) in
 theorem IsDefEqStrong.forallE_inv' (hΓ : CtxStrong env U Γ)
@@ -333,7 +454,7 @@ theorem IsDefEqStrong.forallE_inv' (hΓ : CtxStrong env U Γ)
       refine ⟨⟨_, h4.instN henv hΓ .zero A1 hΓ⟩, _, h4.instN henv hΓ (.succ .zero) A2 ?_⟩
       exact ⟨hΓ, _, h4.instN henv hΓ .zero A1 hΓ⟩
     | _ => cases eq
-  | eta _ _ _ _ _ _ _ _ _ _ ih =>
+  | eta _ _ _ _ _ _ _ _ _ _ _ ih =>
     obtain ⟨⟨⟩⟩ | eq := eq
     exact ih hΓ (.inl eq)
   | @extra df ls _ Γ h1 h2 =>
@@ -345,7 +466,7 @@ theorem IsDefEqStrong.forallE_inv' (hΓ : CtxStrong env U Γ)
       cases eq <;> exact this _ ‹_› ‹_›
     intro e eq IH
     cases e <;> cases eq; rename_i A B
-    let ⟨⟨_, A1⟩, v, A2⟩ := IH.2.2 _ _ rfl
+    let ⟨⟨_, A1⟩, v, A2⟩ := IH.2.2.2 _ _ rfl
     refine ⟨⟨_, (A1.instL h2).weak0 henv⟩, v.inst ls, ?_⟩
     have := (A2.instL h2).weakN henv (.succ (.zero Γ))
     have C1 := (A1.instL h2).defeq.closedN henv ⟨⟩
@@ -373,7 +494,7 @@ theorem IsDefEqStrong.isType' (hΓ : CtxStrong env U Γ) (H : env.IsDefEqStrong 
   | forallEDF h1 h2 => exact ⟨_, .sortDF ⟨h1, h2⟩ ⟨h1, h2⟩ rfl⟩
   | defeqDF _ h2 => exact ⟨_, h2.hasType.2⟩
   | beta _ _ _ h4 _ h6 => exact ⟨_, h6.hasType.1.instN henv hΓ .zero h4 hΓ⟩
-  | eta _ _ _ _ _ _ _ _ _ _ ih => exact ih hΓ
+  | eta _ _ _ _ _ _ _ _ _ _ _ ih => exact ih hΓ
   | proofIrrel h1 => exact ⟨_, h1⟩
   | extra h1 h2 =>
     have ⟨_, h⟩ := (envIH.2 h1).2.2.1
@@ -404,6 +525,86 @@ theorem IsDefEqStrong.instDF
       .defeqDF hv (.symm hi) (H1 hf.hasType.2 ha.hasType.2)
   H2 hv hB hf <| H2 (v := v.succ) hv (.sortDF hv hv rfl) hB (.sortDF hv hv rfl)
 
+variable! (henv : Ordered env) (envIH : env.OnTypes (EnvStrong env))
+  (W : CtxStrong env U Γ) in
+theorem EqUpToLevels.defeq (H : env.IsDefEqStrong U Γ e1 e2 A)
+    (H1 : EqUpToLevels U e1 e1') (H2 : EqUpToLevels U e2 e2') :
+    env.IsDefEqStrong U Γ e1' e2' A := by
+  induction H generalizing e1' e2' with
+  | bvar h1 h2 h3 => let .bvar := H1; let .bvar := H2; exact .bvar h1 h2 h3
+  | constDF h1 h2 h3 h4 h5 h6 _ _ ih1 ih2 =>
+    let .const a1 a2 a3 := H1
+    let .const b1 b2 b3 := H2
+    let ⟨_, c1⟩ := envIH.1 h1
+    have c2 := a3.flip.trans (T := (· ≈ ·)) (fun _ _ _  => (·.symm.trans)) <|
+      h5.trans (T := (· ≈ ·)) (fun _ _ _ => Eq.trans) b3
+    have := c1.2.2.1 _ _ _ a2 b2 c2
+    exact .defeqDF (.inst a1) (.symm ((c1.2.2.1 _ _ _ a1 a2 a3).weak0 henv)) <|
+      .constDF h1 a2 b2 (a3.length_eq.symm.trans h4) c2 (.inst a2) this (this.weak0 henv)
+  | symm _ ih => exact (ih W H2 H1).symm
+  | trans h1 _ ih1 ih2 =>
+    have H3 := (EqUpToLevels.refl W.levelWF h1).2; exact (ih1 W H1 H3).trans (ih2 W H3 H2)
+  | sortDF h1 h2 h3 =>
+    let .sort a1 a2 a3 := H1
+    let .sort b1 b2 b3 := H2
+    exact .defeqDF (by exact a1)
+      (.symm <| .sortDF (by exact a1) (by exact a2) (VLevel.succ_congr a3))
+      (.sortDF a2 b2 (a3.symm.trans <| h3.trans b3))
+  | appDF h1 h2 h3 h4 h5 h6 _ ih1 ih2 ih3 ih4 ih5 =>
+    let .app a1 a2 := H1
+    let .app b1 b2 := H2
+    have := ih4 W a2 (EqUpToLevels.refl W.levelWF h6).2 |>.trans h6.symm
+    exact .defeqDF h2 (.instDF henv W h1 (by exact h2) h3 (.sortDF h2 h2 rfl) h4 this) <|
+      .appDF h1 h2 h3 h4 (ih3 W a1 b1) (ih4 W a2 b2) <|
+      .instDF henv W h1 (by exact h2) h3 (.sortDF h2 h2 rfl) h4 (ih4 W a2 b2)
+  | lamDF h1 h2 h3 h4 h5 h6 h7 ih1 ih2 ih3 ih4 =>
+    let .lam a1 a2 := H1
+    let .lam b1 b2 := H2
+    have c1 := ih1 W a1 (EqUpToLevels.refl W.levelWF h3).2 |>.trans h3.symm
+    have c2 := ih1 W (EqUpToLevels.refl W.levelWF h3).1 b1
+    have h4' := c1.symm.defeqDF_l henv W h4
+    exact have ih := ih4 ⟨W, _, h3.hasType.1⟩ a2 b2
+      .defeqDF (by exact ⟨h1, h2⟩) (.forallEDF h1 h2 c1 h4' h4) <|
+      .lamDF h1 h2 (ih1 W a1 b1) h4' (.defeqDF_l henv W c2 h4)
+        (.defeqDF_l henv W c1.symm ih) (.defeqDF_l henv W c2 ih)
+  | forallEDF h1 h2 h3 _ _ ih1 ih2 =>
+    let .forallE a1 a2 := H1
+    let .forallE b1 b2 := H2
+    have c1 := ih1 W a1 (EqUpToLevels.refl W.levelWF h3).2 |>.trans h3.symm
+    have c2 := ih1 W (EqUpToLevels.refl W.levelWF h3).1 b1
+    exact .forallEDF h1 h2 (ih1 W a1 b1)
+      (.defeqDF_l henv W c1.symm <| ih2 ⟨W, _, h3.hasType.1⟩ a2 b2)
+      (.defeqDF_l henv W c2 <| ih2 ⟨W, _, h3.hasType.1⟩ a2 b2)
+  | defeqDF h1 h2 _ _ ih => exact .defeqDF h1 h2 (ih W H1 H2)
+  | beta h1 h2 h3 h4 h5 h6 h7 _ ih1 _ ih3 ih4 ih5 ih6 =>
+    let .app a1 a3 := H1; let .lam a1 a2 := a1
+    have c1 := ih1 W a1 (EqUpToLevels.refl W.levelWF h3).2 |>.trans h3.symm
+    have c2 := ih4 W a3 (EqUpToLevels.refl W.levelWF h6).2 |>.trans h6.symm
+    have c3 := ih3 ⟨W, _, h3⟩ a2 a2
+    have hb := (EqUpToLevels.refl (CtxStrong.levelWF (by exact ⟨W, _, h3⟩)) h4).2
+    have c4 := ih5 W (.instN a3 hb) (EqUpToLevels.refl W.levelWF h7).2
+    refine .trans ?_ (ih6 W (.instN a3 a2) H2)
+    refine .defeqDF h2 (.instDF henv W h1 (by exact h2) h3 (.sortDF h2 h2 rfl) h4 c2) ?_
+    exact .beta h1 h2 c1.hasType.1 (.defeqDF_l henv W c1.symm h4)
+      (.defeqDF_l henv W c1.symm c3) (.defeqDF h1 c1.symm c2.hasType.1)
+      c4.hasType.1 (.instN henv c2.hasType.1 W .zero c3 W)
+  | eta h1 h2 h3 h4 h5 h6 h7 h8 ih1 ih2 ih3 ih4 ih5 =>
+    let .lam a1 a3 := H1; let .app a2 a3 := a3; let .bvar := a3
+    have c1 := ih1 W a1 (EqUpToLevels.refl W.levelWF h3).2 |>.trans h3.symm
+    have c2 := have W' := ⟨W, _, h3⟩; ih5 W' a2 (EqUpToLevels.refl W'.levelWF h7).2
+    have c3 := IsDefEqStrong.appDF h1 h2 h8 h5 c2 (.bvar .zero h1 h8)
+    rw [instN_bvar0] at c3; specialize c3 h4
+    refine .trans
+      (.symm <| .lamDF h1 h2 c1.symm h4 (.defeqDF_l henv W c1.symm h4) c3.symm
+        (.defeqDF_l henv W c1.symm c3.symm)) ?_
+    exact .trans (.eta h1 h2 h3 h4 h5 h6 h7 h8) (ih4 W (EqUpToLevels.refl W.levelWF h6).1 H2)
+  | proofIrrel h1 _ _ _ ih1 ih2 => exact .proofIrrel h1 (ih1 W H1 H1) (ih2 W H2 H2)
+  | extra h1 h2 h3 h4 h5 h6 h7 h8 h9 _ ih1 ih2 =>
+    have c1 := ih1 trivial H1 (EqUpToLevels.refl (by trivial) h6).2
+    have c2 := ih2 trivial H2 (EqUpToLevels.refl (by trivial) h7).2
+    refine .weak0 henv <| c1.trans <| .trans ?_ c2.symm
+    exact .extra h1 h2 h3 h4 h5 h6 h7 h6 h7
+
 variable! (henv : Ordered env) (envIH : env.OnTypes (EnvStrong env)) in
 theorem IsDefEq.strong' (hΓ : CtxStrong env U Γ)
     (H : env.IsDefEq U Γ e1 e2 A) : env.IsDefEqStrong U Γ e1 e2 A := by
@@ -418,10 +619,8 @@ theorem IsDefEq.strong' (hΓ : CtxStrong env U Γ)
   | sortDF h1 h2 h3 => exact .sortDF h1 h2 h3
   | @constDF _ _ ls₁ ls₂ _ h1 h2 h3 h4 h5 =>
     let ⟨u, h6⟩ := envIH.1 h1
-    have H1 := h6.1.instL h2
-    have H2 := IsDefEqStrong.defeqDF (u := .succ _) (.inst h2)
-      (.symm <| .sortDF (.inst h2) (.inst h3) (VLevel.inst_congr rfl h5)) <| h6.1.instL h3
-    exact .constDF h1 h2 h3 h4 h5 (.inst h2) H1 H2 (H1.weak0 henv) (H2.weak0 henv)
+    have := h6.2.2.1 _ _ _ h2 h3 h5
+    exact .constDF h1 h2 h3 h4 h5 (.inst h2) this (this.weak0 henv)
   | appDF _ _ ih1 ih2 =>
     let ⟨_, h3⟩ := (ih1 hΓ).isType' henv envIH hΓ
     let ⟨⟨u, hA⟩, ⟨v, hB⟩⟩ := h3.forallE_inv' henv envIH hΓ (.inl rfl)
@@ -457,7 +656,7 @@ theorem IsDefEq.strong' (hΓ : CtxStrong env U Γ)
     let ⟨⟨u, hA⟩, ⟨v, hB⟩⟩ := hAB.forallE_inv' henv envIH hΓ (.inl rfl)
     have hΓ' : CtxStrong env U (_::_) := ⟨hΓ, _, hA⟩
     exact .eta (hA.defeq.sort_r henv hΓ.defeq) (hB.defeq.sort_r henv hΓ'.defeq)
-      hA hB (hB.weakN henv (.succ .one)) he (he.weakN henv .one)
+      hA hB (hB.weakN henv (.succ .one)) he (he.weakN henv .one) (hA.weakN henv .one)
   | proofIrrel _ _ _ ih1 ih2 ih3 => exact .proofIrrel (ih1 hΓ) (ih2 hΓ) (ih3 hΓ)
   | extra h1 h2 h3 =>
     let ⟨⟨hl, ⟨_, ht⟩, _⟩, hr, _, _⟩ := envIH.2 h1
@@ -470,13 +669,16 @@ theorem CtxStrong.strong' (henv : Ordered env) (envIH : env.OnTypes (EnvStrong e
   | nil => trivial
   | cons _ _ ih => let ⟨hΓ, _, hA⟩ := hΓ; exact ⟨ih hΓ, _, hA.strong' henv envIH (ih hΓ)⟩
 
-theorem Ordered.strong (henv : Ordered env) : OnTypes env (EnvStrong env) :=
-  henv.induction _
-    (fun le ⟨h1, ⟨_, h2⟩, h3⟩ => ⟨h1.mono le, ⟨_, h2.mono le⟩, fun _ _ eq =>
-      let ⟨⟨_, h4⟩, ⟨_, h5⟩⟩ := h3 _ _ eq; ⟨⟨_, h4.mono le⟩, ⟨_, h5.mono le⟩⟩⟩)
-    (fun henv IH H =>
-      have H' := H.strong' henv IH (Γ := []) ⟨⟩
-      ⟨H', H'.isType' henv IH ⟨⟩, fun _ _ eq => H'.forallE_inv' henv IH ⟨⟩ (.inl eq)⟩)
+theorem Ordered.strong (henv : Ordered env) : OnTypes env (EnvStrong env) := by
+  refine henv.induction _ (fun le ⟨h1, ⟨_, h2⟩, h3, h4⟩ => ?_) (fun henv IH H => ?_)
+  · refine ⟨h1.mono le, ⟨_, h2.mono le⟩, ?_, ?_⟩
+    · exact fun _ _ _ h4 h5 h6 => (h3 _ _ _ h4 h5 h6).mono le
+    · exact fun _ _ eq => let ⟨⟨_, h4⟩, ⟨_, h5⟩⟩ := h4 _ _ eq; ⟨⟨_, h4.mono le⟩, ⟨_, h5.mono le⟩⟩
+  · have H' := H.strong' henv IH (Γ := []) ⟨⟩
+    refine ⟨H', H'.isType' henv IH ⟨⟩, fun _ _ _ h1 h2 h3 => ?_, ?_⟩
+    · exact EqUpToLevels.defeq henv IH (by trivial) (.instL h1 H')
+        (EqUpToLevels.refl (by trivial) (.instL h1 H')).1 (EqUpToLevels.instL h1 h2 h3 H').1
+    · exact fun _ _ eq => H'.forallE_inv' henv IH ⟨⟩ (.inl eq)
 
 theorem CtxStrong.strong (henv : Ordered env) (hΓ : OnCtx Γ (env.IsType U)) : CtxStrong env U Γ :=
   .strong' henv henv.strong hΓ
@@ -505,7 +707,7 @@ theorem IsDefEq.app_inv'
     obtain ⟨⟨⟩⟩ | eq := eq
     · exact ⟨_, _, .lam hA.defeq he.defeq, he'.defeq⟩
     · exact ihee (.inl eq)
-  | eta _ _ _ _ _ _ _ _ _ _ ih =>
+  | eta _ _ _ _ _ _ _ _ _ _ _ ih =>
     obtain ⟨⟨⟩⟩ | eq := eq
     exact ih (.inl eq)
   | _ => nomatch eq
@@ -539,7 +741,7 @@ theorem IsDefEq.lam_inv'
   | beta _ _ _ _ _ _ _ _ _ _ _ _ _ ihee =>
     obtain ⟨⟨⟩⟩ | eq := eq
     exact ihee (.inl eq)
-  | eta _ _ hA _ _ _ he' _ _ _ ih =>
+  | eta _ _ hA _ _ _ he' _ _ _ _ ih =>
     obtain ⟨⟨⟩⟩ | eq := eq
     · exact ⟨⟨_, hA.defeq.hasType.1⟩, _, he'.defeq.hasType.1.app (.bvar .zero)⟩
     · exact ih (.inl eq)
@@ -574,7 +776,7 @@ theorem IsDefEq.const_inv'
   | beta _ _ _ _ _ _ _ _ _ _ _ _ _ ihee =>
     obtain ⟨⟨⟩⟩ | eq := eq
     exact ihee (.inl eq)
-  | eta _ _ _ _ _ _ _ _ _ _ ih =>
+  | eta _ _ _ _ _ _ _ _ _ _ _ ih =>
     obtain ⟨⟨⟩⟩ | eq := eq
     exact ih (.inl eq)
   | _ => nomatch eq
@@ -588,3 +790,169 @@ variable! (henv : Ordered env) (hΓ : OnCtx Γ (env.IsType U)) in
 theorem _root_.Lean4Lean.VExpr.WF.const_inv (H : VExpr.WF env U Γ (.const c ls)) :
     ∃ ci, env.constants c = some ci ∧ (∀ l ∈ ls, l.WF U) ∧ ls.length = ci.uvars :=
   let ⟨_, H⟩ := H; HasType.const_inv henv hΓ H
+
+variable! (henv : Ordered env) (hΓ : OnCtx Γ (env.IsType U)) in
+theorem IsDefEq.eqUpToLevels (H : env.IsDefEq U Γ e1 e2 A)
+    (H1 : EqUpToLevels U e2 e2') : env.IsDefEq U Γ e1 e2' A :=
+  have W := .strong' henv henv.strong hΓ
+  have := H.strong henv hΓ
+  (EqUpToLevels.defeq henv henv.strong W (H.strong henv hΓ)
+    (EqUpToLevels.refl W.levelWF this).1 H1).defeq
+
+variable! (henv : Ordered env) (hΓ : OnCtx Γ (env.IsType U')) {ls ls' : List VLevel}
+    (hls : ∀ l ∈ ls, l.WF U) (hls' : ∀ l ∈ ls', l.WF U) (heq : List.Forall₂ (· ≈ ·) ls ls') in
+theorem IsDefEq.instL_r (H : env.IsDefEq U' Γ e1 e2 A) :
+    env.IsDefEq U (Γ.map (VExpr.instL ls)) (e1.instL ls) (e2.instL ls') (A.instL ls) :=
+  have := H.strong henv hΓ
+  IsDefEq.eqUpToLevels henv (hΓ.instL hls) (this.instL hls).defeq
+    (EqUpToLevels.instL hls hls' heq this).2
+
+theorem IsDefEqStrong.hasType' {env : VEnv}
+    (H : env.IsDefEqStrong U Γ e1 e2 A) :
+    env.HasTypeStrong U Γ e1 A true ∧ env.HasTypeStrong U Γ e2 A true := by
+  induction H with
+  | bvar h1 h2 _ ih3 => refine and_self_iff.2 <| .base <| .bvar h1 h2 ih3.1
+  | symm _ ih => exact ih.symm
+  | trans _ _ ih1 ih2 | proofIrrel _ _ _ _ ih1 ih2 => exact ⟨ih1.1, ih2.2⟩
+  | sortDF h1 h2 h3 => exact ⟨.base <| .sort' h1 h1 rfl, .base <| .sort' h2 h1 h3.symm⟩
+  | constDF h1 h2 h3 h4 h5 h6 h7 h8 ih1 ih2 =>
+    exact ⟨.base <| .const h1 h2 h4 h6 ih1.1 ih2.1,
+      .defeq h6 h8.symm ih2.2 ih2.1 <| .base <|
+      .const h1 h3 (h5.length_eq.symm.trans h4) h6 ih1.2 ih2.2⟩
+  | appDF h1 h2 h3 h4 h5 h6 h7 ih1 ih2 ih3 ih4 ih5 =>
+    have := HasTypeStrong.base <| .forallE h1 h2 ih1.1 ih2.1
+    exact ⟨.base <| .app h1 h2 ih1.1 ih2.1 this ih3.1 ih4.1 ih5.1,
+      .defeq h2 h7.symm ih5.2 ih5.1 <| .base <| .app h1 h2 ih1.2 ih2.2 this ih3.2 ih4.2 ih5.2⟩
+  | lamDF h1 h2 h3 h4 h5 h6 h7 ih1 ih2 ih3 ih4 ih5 =>
+    refine ⟨.base <| .lam h1 h2 ih1.1 ih2.1 ih4.1 ?a,
+      .defeq (by exact ⟨h1, h2⟩) (.symm <| .forallEDF h1 h2 h3 h4 h5) ?b ?a ?_⟩
+    · exact .base <| .forallE h1 h2 ih1.1 ih2.1
+    · exact .base <| .forallE h1 h2 ih1.2 ih3.1
+    · exact .base <| .lam h1 h2 ih1.2 ih3.1 ih5.2 ?b
+  | forallEDF h1 h2 h3 h4 h5 ih1 ih2 ih3 =>
+    exact ⟨.base <| .forallE h1 h2 ih1.1 ih2.1, .base <| .forallE h1 h2 ih1.2 ih3.2⟩
+  | defeqDF h1 h2 h3 ih1 ih2 =>
+    exact ⟨.defeq h1 h2 ih1.1 ih1.2 ih2.1, .defeq h1 h2 ih1.1 ih1.2 ih2.2⟩
+  | beta h1 h2 _ _ _ _ _ _ ih1 ih2 ih3 ih4 ih5 ih6 =>
+    have := HasTypeStrong.base <| .forallE h1 h2 ih1.1 ih2.1
+    refine ⟨.base <| .app h1 h2 ih1.1 ih2.1 this ?_ ih4.1 ih5.1, ih6.1⟩
+    refine .base <| .lam h1 h2 ih1.1 ih2.1 ih3.1 ?_
+    exact .base <| .forallE h1 h2 ih1.1 ih2.1
+  | @eta Γ A u B v e h1 h2 _ _ _ _ _ _ ih1 ih2 ih3 ih4 ih5 ih6 =>
+    refine have a1 := .base <| .forallE h1 h2 ih6.1 ih3.1
+      have := ih6.1.app h1 h2 ih3.1 a1 ih5.1 (.base <| .bvar .zero h1 ih6.1); ?_
+    rw [instN_bvar0] at this; specialize this ih2.1
+    refine ⟨.base <| .lam h1 h2 ih1.1 ih2.1 (.base this) ?_, ih4.1⟩
+    exact .base <| .forallE h1 h2 ih1.1 ih2.1
+  | extra h1 h2 h3 h4 h5 h6 h7 _ _ _ _ _ ih4 ih5 => exact ⟨ih4.1, ih5.1⟩
+
+theorem HasTypeStrong.refl {env : VEnv}
+    (H : env.HasTypeStrong U Γ e A b) : env.IsDefEqStrong U Γ e e A := by
+  induction H with
+  | bvar h1 h2 _ ih1 => refine .bvar h1 h2 ih1
+  | sort' h1 h2 h3 =>
+    refine .defeqDF ?_ (.sortDF ?_ ?_ (VLevel.succ_congr h3)) (.sortDF h1 h1 rfl) <;> assumption
+  | const h1 h2 h3 h4 h5 h6 ih1 ih2 =>
+    exact .constDF h1 h2 h2 h3 (.rfl fun _ _ => rfl) h4 ih1 ih2
+  | app h1 h2 h3 h4 _ h5 h6 h7 ih1 ih2 _ ih3 ih4 ih5 =>
+    exact .appDF h1 h2 ih1 ih2 ih3 ih4 ih5
+  | lam h1 h2 h3 h4 h5 _ ih1 ih2 ih3 =>
+    exact .lamDF h1 h2 ih1 ih2 ih2 ih3 ih3
+  | forallE h1 h2 h3 h4 ih1 ih2 =>
+    exact .forallEDF h1 h2 ih1 ih2 ih2
+  | base _ ih => exact ih
+  | defeq h1 h2 h3 h4 h5 ih1 ih2 ih3 => exact .defeqDF h1 h2 ih3
+
+theorem HasTypeStrong.hasType {env : VEnv}
+    (H : env.HasTypeStrong U Γ e A b) :  env.HasType U Γ e A := H.refl.defeq.hasType.1
+
+set_option hygiene false
+local notation:65 Γ " ⊢ " e " : " A:36 => HasType env U Γ e A
+local notation:65 Γ " ⊢ " e1 " ≡ " e2 " : " A:36 => IsDefEq env U Γ e1 e2 A
+section
+local notation:65 Γ " ⊢ " e " : " A " !! " n:30 => HasTypeStratified Γ e A true n
+local notation:65 Γ " ⊢ " e " :! " A " !! " n:30 => HasTypeStratified Γ e A false n
+
+variable (env : VEnv) (U : Nat) in
+inductive HasTypeStratified : List VExpr → VExpr → VExpr → Bool → Nat → Prop where
+  | bvar : Lookup Γ i A → Γ ⊢ A : .sort u !! n → Γ ⊢ .bvar i :! A !! n+1
+  | sort' : l.WF U → l'.WF U → l ≈ l' → Γ ⊢ .sort l :! .sort (.succ l') !! n
+  | const :
+    env.constants c = some ci →
+    (∀ l ∈ ls, l.WF U) →
+    ls.length = ci.uvars →
+    Γ ⊢ ci.type.instL ls : .sort u !! n →
+    Γ ⊢ .const c ls :! ci.type.instL ls !! n+1
+  | app :
+    u.WF U → v.WF U →
+    Γ ⊢ A : .sort u !! n →
+    A::Γ ⊢ B : .sort v !! n →
+    Γ ⊢ f : .forallE A B !! n →
+    Γ ⊢ a : A !! n →
+    Γ ⊢ B.inst a : .sort v !! n →
+    Γ ⊢ .app f a :! B.inst a !! n+1
+  | lam :
+    Γ ⊢ A : .sort u !! n →
+    A::Γ ⊢ B : .sort v !! n →
+    A::Γ ⊢ body : B !! n →
+    Γ ⊢ .forallE A B : .sort (.imax u v) !! n →
+    Γ ⊢ .lam A body :! .forallE A B !! n+1
+  | forallE :
+    u.WF U → v.WF U →
+    Γ ⊢ A : .sort u !! n →
+    A::Γ ⊢ body : .sort v !! n →
+    Γ ⊢ .forallE A body :! .sort (.imax u v) !! n+1
+  | base : Γ ⊢ e :! A !! n → Γ ⊢ e : A !! n
+  | defeq : u.WF U → Γ ⊢ A ≡ B : .sort u →
+    Γ ⊢ A : .sort u !! n → Γ ⊢ B : .sort u !! n → Γ ⊢ e : A !! n → Γ ⊢ e : B !! n+1
+end
+
+theorem HasTypeStratified.hasType (H : env.HasTypeStratified U Γ e A b n) : Γ ⊢ e : A := by
+  induction H with
+  | bvar h1 h2 ih1 => refine .bvar h1
+  | sort' h1 h2 h3 =>
+    exact IsDefEq.defeq (.sortDF (by exact h1) h2 (VLevel.succ_congr h3)) (.sort h1)
+  | const h1 h2 h3 => exact .const h1 h2 h3
+  | app _ _ _ _ _ _ _ _ _ ih3 ih4 => exact .app ih3 ih4
+  | lam _ _ _ _ ih1 _ ih3 => exact .lam ih1 ih3
+  | forallE _ _ _ _ ih1 ih2 => exact .forallE ih1 ih2
+  | base _ ih => exact ih
+  | defeq _ h2 _ _ _ _ _ ih3 => exact h2.defeq ih3
+
+theorem HasTypeStratified.mono (le : m ≤ n) (H : HasTypeStratified env U Γ e A b m) :
+    env.HasTypeStratified U Γ e A b n := by
+  induction H generalizing n with try let n+1 := n; replace le := Nat.le_of_succ_le_succ le
+  | bvar h1 h2 ih1 => exact .bvar h1 (ih1 le)
+  | sort' h1 h2 h3 => exact .sort' h1 h2 h3
+  | const h1 h2 h3 _ ih1 => exact .const h1 h2 h3 (ih1 le)
+  | app h1 h2 _ _ _ _ _ ih1 ih2 ih3 ih4 ih5 =>
+    exact .app h1 h2 (ih1 le) (ih2 le) (ih3 le) (ih4 le) (ih5 le)
+  | lam _ _ _ _ ih1 ih2 ih3 ih4 => exact .lam (ih1 le) (ih2 le) (ih3 le) (ih4 le)
+  | forallE h1 h2 _ _ ih1 ih2 => exact .forallE h1 h2 (ih1 le) (ih2 le)
+  | base _ ih => exact .base (ih le)
+  | defeq h1 h2 _ _ _ ih1 ih2 ih3 => exact .defeq h1 h2 (ih1 le) (ih2 le) (ih3 le)
+
+theorem HasTypeStrong.stratify (H : HasTypeStrong env U Γ e A b) :
+    ∃ n, HasTypeStratified env U Γ e A b n := by
+  generalize true = b at H ⊢
+  induction H with
+  | bvar h1 h2 _ ih1 => let ⟨n, ih1⟩ := ih1; exact ⟨_, .bvar h1 ih1⟩
+  | sort' h1 h2 h3 => exact ⟨0, .sort' h1 h2 h3⟩
+  | const h1 h2 h3 _ _ _ _ ih1 => let ⟨_, ih1⟩ := ih1; exact ⟨_, .const h1 h2 h3 ih1⟩
+  | app h1 h2 _ _ _ _ _ _ ih1 ih2 _ ih3 ih4 ih5 =>
+    let ⟨n₁, ih1⟩ := ih1; let ⟨n₂, ih2⟩ := ih2; let ⟨n₃, ih3⟩ := ih3
+    let ⟨n₄, ih4⟩ := ih4; let ⟨n₅, ih5⟩ := ih5
+    refine ⟨max n₁ (max n₂ (max n₃ (max n₄ n₅))) + 1,
+      .app h1 h2 (ih1.mono ?_) (ih2.mono ?_) (ih3.mono ?_) (ih4.mono ?_) (ih5.mono ?_)⟩ <;> omega
+  | lam _ _ _ _ _ _ ih1 ih2 ih3 ih4 =>
+    let ⟨n₁, ih1⟩ := ih1; let ⟨n₂, ih2⟩ := ih2; let ⟨n₃, ih3⟩ := ih3; let ⟨n₄, ih4⟩ := ih4
+    refine ⟨max n₁ (max n₂ (max n₃ n₄)) + 1,
+      .lam (ih1.mono ?_) (ih2.mono ?_) (ih3.mono ?_) (ih4.mono ?_)⟩ <;> omega
+  | forallE h1 h2 _ _ ih1 ih2 =>
+    let ⟨n₁, ih1⟩ := ih1; let ⟨n₂, ih2⟩ := ih2
+    refine ⟨max n₁ n₂ + 1, .forallE h1 h2 (ih1.mono ?_) (ih2.mono ?_)⟩ <;> omega
+  | base _ ih => let ⟨_, ih⟩ := ih; exact ⟨_, .base ih⟩
+  | defeq h1 h2 _ _ _ ih1 ih2 ih3 =>
+    let ⟨n₁, ih1⟩ := ih1; let ⟨n₂, ih2⟩ := ih2; let ⟨n₃, ih3⟩ := ih3
+    refine ⟨max n₁ (max n₂ n₃) + 1,
+      .defeq h1 h2.defeq (ih1.mono ?_) (ih2.mono ?_) (ih3.mono ?_)⟩ <;> omega
