Lean4Lean/Theory/Typing/Injectivity.lean
@@ -1,0 +1,28 @@
+import Lean4Lean.Theory.Typing.EnvLemmas
+import Lean4Lean.Theory.Typing.Strong
+
+/-!
+A bunch of important structural theorems which we can't prove :(
+-/
+
+namespace Lean4Lean
+namespace VEnv
+
+theorem IsDefEqU.sort_inv (henv : VEnv.WF env) (hΓ : OnCtx Γ (env.IsType U))
+    (h1 : env.IsDefEqU U Γ (.sort u) (.sort v)) : u ≈ v := sorry
+
+theorem IsDefEqU.forallE_inv_stratified (henv : VEnv.WF env) (hΓ : OnCtx Γ (env.IsType U))
+    (h1 : env.IsDefEqU U Γ (.forallE A B) (.forallE A' B'))
+    (h2 : env.HasTypeStratified U Γ (.forallE A B) V true n)
+    (h3 : env.HasTypeStratified U Γ (.forallE A' B') V' true n') :
+    (∃ u, env.IsDefEq U Γ A A' (.sort u) ∧ env.HasTypeStratified U Γ A (.sort u) true n) ∧
+    ∃ u, env.IsDefEq U (A::Γ) B B' (.sort u) ∧
+      env.HasTypeStratified U (A::Γ) B (.sort u) true n ∧
+      env.HasTypeStratified U (A'::Γ) B' (.sort u) true n' := sorry
+
+theorem IsDefEqU.forallE_inv (henv : VEnv.WF env) (hΓ : OnCtx Γ (env.IsType U))
+    (h1 : env.IsDefEqU U Γ (.forallE A B) (.forallE A' B')) :
+    (∃ u, env.IsDefEq U Γ A A' (.sort u)) ∧ ∃ u, env.IsDefEq U (A::Γ) B B' (.sort u) := sorry
+
+theorem IsDefEqU.sort_forallE_inv (henv : VEnv.WF env) (hΓ : OnCtx Γ (env.IsType U)) :
+    ¬env.IsDefEqU U Γ (.sort u) (.forallE A B) := sorry
