Lean4Lean/Theory/Typing/UniqueTyping.lean
@@ -1,28 +1,121 @@
-import Lean4Lean.Theory.Typing.Lemmas
-import Lean4Lean.Theory.Typing.EnvLemmas
+import Lean4Lean.Theory.Typing.Injectivity
+import Lean4Lean.Theory.Typing.Pattern
 
-/-!
-A bunch of important structural theorems which we can't prove :(
--/
+/-! # Unique typing and its consequences. -/
 
 namespace Lean4Lean
 namespace VEnv
 
+variable {env : VEnv} {U : Nat}
+local notation:65 Γ " ⊢ " e " : " A:36 => HasType env U Γ e A
+local notation:65 Γ " ⊢ " e1 " ≡ " e2 " : " A:36 => IsDefEq env U Γ e1 e2 A
+
 theorem IsDefEq.uniq (henv : VEnv.WF env) (hΓ : OnCtx Γ (env.IsType U))
-    (h1 : env.IsDefEq U Γ e₁ e₂ A) (h2 : env.IsDefEq U Γ e₂ e₃ B) :
-    ∃ u, env.IsDefEq U Γ A B (.sort u) := sorry
+    (h1 : Γ ⊢ e₁ ≡ e₂ : A) (h2 : Γ ⊢ e₂ ≡ e₃ : B) : ∃ u, Γ ⊢ A ≡ B : .sort u := by
+  suffices ∀ {e A B b n₁ n₂ n}, n₁ ≤ n → n₂ ≤ n →
+      env.HasTypeStratified U Γ e A b n₁ → env.HasTypeStratified U Γ e B b n₂ →
+      ∃ u, Γ ⊢ A ≡ B : .sort u ∧ ∃ v, u ≈ v ∧
+        env.HasTypeStratified U Γ A (.sort u) true (n-1) ∧
+        env.HasTypeStratified U Γ B (.sort v) true (n-1) from
+    let ⟨n₁, h1⟩ := (h1.strong henv hΓ).hasType'.2.stratify
+    let ⟨n₂, h2⟩ := (h2.strong henv hΓ).hasType'.1.stratify
+    have ⟨_, h, _⟩ := this (Nat.le_max_left ..) (Nat.le_max_right ..) h1 h2
+    ⟨_, h⟩
+  clear h1 h2; intro e A B b n₁ n₂ n le₁ le₂ H1
+  induction n using WellFounded.induction Nat.lt_wfRel.2
+    generalizing n₁ n₂ Γ e A B b with | _ n IH
+  dsimp [Nat.lt_wfRel] at IH
+  induction H1 generalizing B n₂ n with
+  | bvar a1 a2 =>
+    intro (.bvar b1 b2); cases a1.uniq b1
+    exact ⟨_, b2.hasType, _, rfl, b2.mono (by omega), b2.mono (by omega)⟩
+  | sort' a1 a2 a3 =>
+    intro (.sort' b1 b2 b3)
+    have := VLevel.succ_congr (b3.symm.trans a3)
+    exact ⟨_, .symm <| .sortDF b2 a2 this, _, VLevel.succ_congr this,
+      .base <| .sort' a2 b2 this.symm, .base <| .sort' b2 a2 this⟩
+  | const a1 a2 a3 a4 =>
+    intro (.const b1 b2 b3 b4); cases a1.symm.trans b1
+    replace le₁ := Nat.sub_le_sub_right le₁ 1
+    exact ⟨_, a4.hasType, _, rfl, a4.mono le₁, a4.mono le₁⟩
+  | app a1 a2 a3 a4 a5 a6 a7 ih1 ih2 ih3 ih4 ih5 =>
+    intro (.app b1 b2 b3 b4 b5 b6 b7)
+    have ⟨_, c1, _, c2, c3, c4⟩ := ih3 n IH hΓ (Nat.le_of_succ_le le₁) (Nat.le_of_succ_le le₂) b5
+    have ⟨⟨_, d1, d2⟩, _, d3, d4, d5⟩ := IsDefEqU.forallE_inv_stratified henv hΓ ⟨_, c1⟩ c3 c4
+    let n+1 := n
+    replace le₁ := Nat.le_of_succ_le_succ le₁
+    replace le₂ := Nat.le_of_succ_le_succ le₂
+    have e1 := have ⟨_, h⟩ := a3.hasType.isType henv hΓ; h.sort_inv henv
+    have e2 := have ⟨_, h⟩ := b3.hasType.isType henv hΓ; h.sort_inv henv
+    refine have hΓ₁ := ⟨hΓ, _, a3.hasType⟩
+      have ⟨_, h, _⟩ := IH _ (Nat.lt_succ_self _) hΓ₁ le₁ (Nat.le_refl _) a4 d4; ?_
+    have e3 := IsDefEqU.sort_inv henv hΓ₁ ⟨_, h⟩
+    have e4 := have ⟨_, h⟩ := d4.hasType.isType henv hΓ₁; h.sort_inv henv
+    refine have hΓ₂ := ⟨hΓ, _, b3.hasType⟩
+      have ⟨_, h, _⟩ := IH _ (Nat.lt_succ_self _) hΓ₂ le₂ (Nat.le_refl _) b4 d5; ?_
+    have e5 := IsDefEqU.sort_inv henv hΓ₂ ⟨_, h⟩
+    exact ⟨_, .defeqDF (.sortDF e4 a2 e3.symm) (d3.instN henv a6.hasType .zero), _,
+      e3.trans e5.symm, a7.mono le₁, b7.mono le₂⟩
+  | lam a1 a2 a3 a4 ih1 ih2 ih3 ih4 =>
+    intro (.lam b1 b2 b3 b4)
+    have ⟨_, c1, _, c2, c3, c4⟩ := ih3 n IH ⟨hΓ, _, a1.hasType⟩
+      (Nat.le_of_succ_le le₁) (Nat.le_of_succ_le le₂) b3
+    let n+1 := n
+    replace le₁ := Nat.le_of_succ_le_succ le₁
+    replace le₂ := Nat.le_of_succ_le_succ le₂
+    have ⟨_, h, _⟩ := IH _ (Nat.lt_succ_self _) hΓ le₁ le₂ a1 b1
+    have e1 := IsDefEqU.sort_inv henv hΓ ⟨_, h⟩
+    refine have hΓ' := ⟨hΓ, _, a1.hasType⟩
+      have ⟨_, h, _⟩ := IH _ (Nat.lt_succ_self _) hΓ' le₁ (Nat.le_refl _) a2 c3; ?_
+    have f1 := h.sort_inv_l henv; have f2 := h.sort_inv_r henv
+    have e2 := IsDefEqU.sort_inv henv hΓ' ⟨_, h⟩
+    have ⟨_, h, _⟩ := IH _ (Nat.lt_succ_self _) hΓ' le₂ (Nat.le_refl _) b2 c4
+    have e3 := IsDefEqU.sort_inv henv hΓ' ⟨_, h⟩
+    exact ⟨_, .forallEDF a1.hasType (.defeqDF (.symm <| .sortDF f1 f2 e2) c1),
+      _, VLevel.imax_congr e1 (e2.trans <| c2.trans e3.symm), a4.mono le₁, b4.mono le₂⟩
+  | forallE a1 a2 a3 a4 ih1 ih2 =>
+    intro (.forallE b1 b2 b3 b4)
+    let n+1 := n
+    replace le₁ := Nat.le_of_succ_le_succ le₁
+    replace le₂ := Nat.le_of_succ_le_succ le₂
+    have ⟨_, h, _⟩ := IH _ (Nat.lt_succ_self _) hΓ le₁ le₂ a3 b3
+    have e1 := IsDefEqU.sort_inv henv hΓ ⟨_, h⟩
+    refine have hΓ' := ⟨hΓ, _, a3.hasType⟩
+      have ⟨_, h, _⟩ := IH _ (Nat.lt_succ_self _) hΓ' le₁ le₂ a4 b4; ?_
+    have f1 := h.sort_inv_l henv; have f2 := h.sort_inv_r henv
+    have e2 := IsDefEqU.sort_inv henv hΓ' ⟨_, h⟩
+    have := VLevel.imax_congr e1 e2
+    exact ⟨_, .sortDF ⟨a1, a2⟩ ⟨b1, b2⟩ this, _, rfl,
+      .base <| .sort' ⟨a1, a2⟩ ⟨a1, a2⟩ rfl, .base <| .sort' ⟨b1, b2⟩ ⟨a1, a2⟩ this.symm⟩
+  | @base Γ e A n₁ a1 ih =>
+    intro H2
+    replace ih {n'} le := @ih n' (fun y h1 => IH y (Nat.lt_of_lt_of_le h1 le)) hΓ
+    generalize eq : true = b at H2
+    induction H2 with cases eq
+    | @base _ _  _ n' b1 => exact ih (Nat.le_refl _) le₁ le₂ b1
+    | @defeq Γ B' B u n' _ b1 b2 b3 b4 b5 _ _ ih' =>
+      have ⟨u₁, c1, u₂, c2, c3, c4⟩ := ih' a1 hΓ (Nat.le_of_succ_le le₂) ih rfl
+      let n+1 := n
+      replace le₂ := Nat.le_of_succ_le_succ le₂
+      have ⟨v₁, d1, v₂, _⟩ := IH _ (Nat.lt_succ_self _) hΓ le₂ (Nat.le_refl _) b3 c4
+      have e1 := IsDefEqU.sort_inv henv hΓ ⟨_, d1⟩
+      have e2 := have ⟨_, h⟩ := c3.hasType.isType henv hΓ; h.sort_inv henv
+      have eq : u₁ ≈ u := c2.trans e1.symm
+      exact ⟨_, c1.trans (.defeqDF (.symm <| .sortDF e2 b1 eq) b2), _, eq, c3, b4.mono le₂⟩
+  | @defeq Γ A' A u n' _ a1 a2 a3 a4 a5 ih1 ih2 ih' =>
+    intro H2
+    have ⟨u₁, c1, u₂, c2, c3, c4⟩ := ih' _ IH hΓ (Nat.le_of_succ_le le₁) le₂ H2
+    let n+1 := n
+    replace le₁ := Nat.le_of_succ_le_succ le₁
+    have ⟨v₁, d1, v₂, _⟩ := IH _ (Nat.lt_succ_self _) hΓ le₁ (Nat.le_refl _) a3 c3
+    have e1 := IsDefEqU.sort_inv henv hΓ ⟨_, d1⟩
+    have e2 := have ⟨_, h⟩ := c3.hasType.isType henv hΓ; h.sort_inv henv
+    have eq : u ≈ u₂ := e1.trans c2
+    exact ⟨_, a2.symm.trans (.defeqDF (.symm <| .sortDF a1 e2 e1) c1), _, eq, a4.mono le₁, c4⟩
 
 theorem IsDefEq.uniqU (henv : VEnv.WF env) (hΓ : OnCtx Γ (env.IsType U))
     (h1 : env.IsDefEq U Γ e₁ e₂ A) (h2 : env.IsDefEq U Γ e₂ e₃ B) :
     env.IsDefEqU U Γ A B := let ⟨_, h⟩ := h1.uniq henv hΓ h2; ⟨_, h⟩
-
-variable! (henv : VEnv.WF env) in
-theorem IsDefEqU.weakN (W : Ctx.LiftN n k Γ Γ') (H : env.IsDefEqU U Γ e1 e2) :
-    env.IsDefEqU U Γ' (e1.liftN n k) (e2.liftN n k) := let ⟨_, H⟩ := H; ⟨_, H.weakN henv W⟩
-
-variable! (henv : VEnv.WF env) in
-theorem IsDefEqU.weak' (W : Ctx.Lift' n Γ Γ') (H : env.IsDefEqU U Γ e1 e2) :
-    env.IsDefEqU U Γ' (e1.lift' n) (e2.lift' n) := let ⟨_, H⟩ := H; ⟨_, H.weak' henv W⟩
 
 theorem isDefEq_iff (henv : VEnv.WF env) (hΓ : OnCtx Γ (env.IsType U)) :
     env.IsDefEq U Γ e₁ e₂ A ↔
@@ -73,16 +166,6 @@ theorem HasType.defeqU_r (henv : VEnv.WF env) (hΓ : OnCtx Γ (env.IsType U))
 theorem IsDefEqU.trans (henv : VEnv.WF env) (hΓ : OnCtx Γ (env.IsType U))
     (h1 : env.IsDefEqU U Γ e₁ e₂) (h2 : env.IsDefEqU U Γ e₂ e₃) :
     env.IsDefEqU U Γ e₁ e₃ := h1.imp fun _ h1 => let ⟨_, h2⟩ := h2; h1.trans_l henv hΓ h2
-
-theorem IsDefEqU.sort_inv (henv : VEnv.WF env) (hΓ : OnCtx Γ (env.IsType U))
-    (h1 : env.IsDefEqU U Γ (.sort u) (.sort v)) : u ≈ v := sorry
-
-theorem IsDefEqU.forallE_inv (henv : VEnv.WF env) (hΓ : OnCtx Γ (env.IsType U))
-    (h1 : env.IsDefEqU U Γ (.forallE A B) (.forallE A' B')) :
-    (∃ u, env.IsDefEq U Γ A A' (.sort u)) ∧ ∃ u, env.IsDefEq U (A::Γ) B B' (.sort u) := sorry
-
-theorem IsDefEqU.sort_forallE_inv (henv : VEnv.WF env) (hΓ : OnCtx Γ (env.IsType U)) :
-    ¬env.IsDefEqU U Γ (.sort u) (.forallE A B) := sorry
 
 variable! (henv : VEnv.WF env) (hΓ : OnCtx Γ' (env.IsType U)) in
 theorem IsDefEqU.weakN_iff (W : Ctx.LiftN n k Γ Γ') :
